show how equality can be solved

MLIR/Examples/EndToEndDiff.lean
@@ -1,4 +1,5 @@
 import MLIR.AST
+import MLIR.EDSL
 
 open MLIR.AST
 
@@ -12,47 +13,118 @@ inductive OpVerifier where
 
 
 inductive OpValid: OpVerifier -> Op -> Prop where
+| MinArgs: ∀ (o: Op) (n: Nat) (PRF: (Op.args o).length >= n),  OpValid (OpVerifier.MinArgs n) o
+| MaxArgs: ∀ (o: Op) (n: Nat) (PRF: (Op.args o).length <= n),  OpValid (OpVerifier.MaxArgs n) o
+| ExactArgs: ∀ (o: Op) (n: Nat) (PRF: (Op.args o).length == n),  OpValid (OpVerifier.ExactArgs n) o
+| And: ∀ (op: Op) (l: OpVerifier) (r: OpVerifier)
+    (PRFL: OpValid l op) (PRFR: OpValid r op), OpValid (OpVerifier.And l r) op
 | True: ∀ (o: Op), OpValid OpVerifier.T o
 
 
--- | proof carrying typed operations 94
-structure OpT (Ops: Type) [Coe Ops String] (Verifier: Ops -> OpVerifier): Type where
-    (kind: Ops) 
+def opValid (o: Op): OpVerifier  -> Bool
+| OpVerifier.T => true
+| OpVerifier.MinArgs n => (Op.args o).length >= n
+| OpVerifier.MaxArgs n => (Op.args o).length <=  n
+| OpVerifier.ExactArgs n => (Op.args o).length == n
+| OpVerifier.And v v' => opValid o v && opValid o v'
+| OpVerifier.MinRegions n => (Op.regions o).length >= n
+
+
+-- | reflection principle for opValid
+-- | TODO: need someone who has done proofs in lean.
+theorem opValid_implies_OpValid: ∀ (v: OpVerifier) (o: Op)(VALID: opValid o v = True), OpValid v o := 
+   sorry
+
+
+@[simp]
+class Verifier (Ops : Type) where
+  verifier : Ops -> OpVerifier
+
+
+-- | proof carrying typed operations
+structure OpT (Ops: Type) [Coe Ops String] [Verifier Ops]: Type where
+    (kind: Ops)
     (args: List SSAVal)
     (bbs: List BBName)
     (regions: List Region) 
     (attrs: AttrDict)
     (ty: MLIRTy)
-    (VALID: OpValid (Verifier kind) (Op.mk kind args bbs regions attrs ty))
+    (VALID: OpValid (Verifier.verifier kind) (Op.mk kind args bbs regions attrs ty))
+
+
+syntax ident  "(" mlir_op_operand,* ")" 
+  ("[" mlir_op_successor_arg,* "]")? ("(" mlir_region,* ")")?  ("{" mlir_attr_entry,* "}")? ":" mlir_type : mlir_op
+
+macro_rules
+  | `([mlir_op|  $opty:ident
+        ( $operands,* )
+        $[ [ $succ,* ] ]?
+        $[ ( $rgns,* ) ]?
+        $[ { $attrs,* } ]? : $ty:mlir_type ]) => do
+        let initList <- `([])
+        let operandsList <- operands.getElems.foldlM (init := initList) fun xs x => `($xs ++ [[mlir_op_operand| $x]])
+        let succList <- match succ with
+                | none => `([])
+                | some xs => xs.getElems.foldlM (init := initList) fun xs x => `($xs ++ [[mlir_op_successor_arg| $x] ])
+        let attrsList <- match attrs with 
+                          | none => `([]) 
+                          | some attrs => attrs.getElems.foldlM (init := initList) fun xs x => `($xs ++ [[mlir_attr_entry| $x]])
+        let rgnsList <- match rgns with 
+                          | none => `([]) 
+                          | some rgns => rgns.getElems.foldlM (init := initList) fun xs x => `($xs ++ [[mlir_region| $x]])
+        `(OpT.mk $opty
+                $operandsList -- operands
+                $succList -- bbs
+                $rgnsList -- regions
+                (AttrDict.mk $attrsList) -- attrs
+                [mlir_type| $ty]) -- type
+
+
 
 inductive DiffOps where
-| var
-| add
-| mul
-| sin
-| d
-
-def DiffVerifier: DiffOps -> OpVerifier
-| DiffOps.var => OpVerifier.ExactArgs 1 
-| DiffOps.add => OpVerifier.ExactArgs 2
-| _ => OpVerifier.T
+| var | add | mul | d
 
 
 
-inductive RewriterT (Ops: Type) (Verifier: Ops -> OpVerifier)
- where
-| op: (ty: Ops) -> (args: List SSAVal) -> (SSAVal -> RewriterT Ops Verifier) -> RewriterT Ops Verifier
-| result: (op: SSAVal) -> (ix: Nat) -> (SSAVal -> RewriterT  Ops Verifier) -> RewriterT Ops Verifier
-| operand:  (SSAVal -> RewriterT Ops Verifier) -> RewriterT Ops Verifier -- fresh operand
-| rewrite: RewriterT Ops Verifier -> RewriterT Ops Verifier -- begin a rewrite block
+instance : Coe DiffOps String where
+  coe: DiffOps -> String
+  | DiffOps.var => "var"
+  | DiffOps.add => "add"
+  | DiffOps.mul => "mul"
+  | DiffOps.d => "d"
+
+@[simp]
+instance : Verifier DiffOps where
+  verifier : DiffOps -> OpVerifier
+  | DiffOps.var => OpVerifier.ExactArgs 0
+  | DiffOps.add => OpVerifier.ExactArgs 2
+  | _ => OpVerifier.T
+
+
+
+-- | diff operation, with num. args checked.
+def diff0 : OpT DiffOps := 
+   let VALID : _ := by {  constructor; simp; }
+   [mlir_op| DiffOps.add (%x, %y) : i32] VALID
+
+#check diff0
+
+
+
+
+inductive RewriterT (Ops: Type) where
+| op: (ty: Ops) -> (args: List SSAVal) -> (SSAVal -> RewriterT Ops) -> RewriterT Ops
+| result: (op: SSAVal) -> (ix: Nat) -> (SSAVal -> RewriterT  Ops) -> RewriterT Ops
+| operand:  (SSAVal -> RewriterT Ops) -> RewriterT Ops -- fresh operand
+| rewrite: RewriterT Ops -> RewriterT Ops -- begin a rewrite block
 | replace: (old: SSAVal) -> (new: SSAVal) 
-   -> RewriterT Ops Verifier -> RewriterT Ops Verifier
-| done: RewriterT Ops Verifier
+   -> RewriterT Ops -> RewriterT Ops
+| done: RewriterT Ops 
 
 
 
 -- | d(x, add(p, q)) = add(d(x, p), d(x, q))
-def DiffOpsPushAdd0: RewriterT DiffOps DiffVerifier := 
+def DiffOpsPushAdd0: RewriterT DiffOps  := 
   RewriterT.op DiffOps.var [] $ λ x => 
   RewriterT.op DiffOps.var [] $ λ p => 
   RewriterT.op DiffOps.var [] $ λ q => 
@@ -71,18 +143,19 @@ inductive interactive: (a: Type k) -> a -> a -> Type (k+1) where
 | layer: (f: a -> a) -> (r: interactive a (f w) v) -> interactive a w (f v)
 
 
+/-
 -- | a proxy to show the value v
 inductive Proxy {t: Type} (v: t) where
 | proxy: Proxy v
 
-inductive RewriterTBuilderProxy (Ops: Type) (Verifier: Ops -> OpVerifier): Type where
   --  (RewriterT Ops Verifier) -> Type where
 | op: (ty: Ops) -> (args: List SSAVal) -> 
-      (rest: @Proxy (RewriterT Ops Verifier) (RewriterT.op ty args (fun _ => RewriterT.done))
+      (rest: @Proxy (RewriterT Ops) (RewriterT.op ty args (fun _ => RewriterT.done))
              -> SSAVal
              -> RewriterTBuilderProxy Ops Verifier)
       -> RewriterTBuilderProxy Ops Verifier
 
+-/
 
 -- | using framework
 /-
@@ -103,7 +176,7 @@ inductive RewriterTBuilderIndexed (Ops: Type) (Verifier: Ops -> OpVerifier):
       -> (rest: SSAVal -> RewriterTBuilderIndexed
       -> RewriterTBuilderIndexed Ops Verifier RewriterT.done
                
--- | using framework
+ -- | using framework
 def DiffOpsPushAddIndexed: Σ r, RewriterTBuilderIndexed DiffOps DiffVerifier r  := by {
   apply RewriterTBuilderIndexed.op DiffOps.add [];
   intros x;
